some changes.

src/beta.v
@@ -1,49 +1,93 @@
 From MPSTCoq Require Export src.unscoped src.expressions src.processes src.sessions.
-Require Import List String Relations.
+Require Import List String Relations ZArith.
+Require Import Setoid Morphisms Coq.Program.Basics.
+Import ListNotations.
 
-Fixpoint find_proc (l: label) (lst: list (label*expr*process)): option (expr*process) :=
-  match lst with
-    | nil                     => Datatypes.None
-    | pair (pair u e) p :: xs => if eqb l u then Datatypes.Some (pair e p) else find_proc l xs 
-  end.
+Inductive betaP: relation session :=
+  | r_comm  : forall p q xs l e Q M,
+              let v := eval_expr e in
+              betaP ((p <-- p_recv q xs) ||| (q <-- p_send p l e Q) ||| M)
+                    ((p <-- subst_expr_proc (p_recv q xs) l v) ||| (q <-- Q) ||| M)
+  | rt_ite  : forall p P Q M,
+              betaP ((p <-- p_ite (e_val (vbool true)) P Q) ||| M) ((p <-- P) ||| M)
+  | rf_ite  : forall p P Q M,
+              betaP ((p <-- p_ite (e_val (vbool false)) P Q) ||| M) ((p <-- Q) ||| M)
+  | r_struct: forall M1 M1' M2 M2', scong M1 M1' -> scong M2' M2 -> betaP M1' M2' -> betaP M1 M2.
 
-Definition beta (s: session): session :=
-  match s with
-    | s_cons (s_cons (s_par p1 (p_recv q1 l)) (s_par q2 (p_send p2 lbl e Q))) M =>
-      if andb (andb (eqb p1 p2) (eqb q1 q2)) (negb (eqb p1 q1))
-      then
-        let v  := eval_expr e in
-        let rp := find_proc lbl l in
-        match rp with
-          | Datatypes.None             => s
-          | Datatypes.Some (pair ej pj) => 
-            match ej with
-               | e_var x => s_cons (s_cons (s_par p1 (subst_expr_proc pj x v)) (s_par q1 Q)) M
-               | _       => s
-            end
-        end
-      else s
-    | _  => s
-  end.
+Declare Instance Equivalence_beta : Equivalence betaP.
 
-Inductive betaI: relation session :=
-  | r_comm: forall p l q lbl e Q M x v rp ej pj,
-            v  = eval_expr e ->
-            rp = find_proc lbl l ->
-            let rp := Datatypes.Some (pair ej pj) in
-            ej = e_var x ->
-            betaI (s_cons (s_cons (s_par p (p_recv q l)) (s_par q (p_send p lbl e Q))) M)
-                  (s_cons (s_cons (s_par p (subst_expr_proc pj x v)) (s_par q Q)) M)
-  | t_cond: forall p e P Q M, 
-            eval_expr e = e_val (tbool true) ->
-            betaI (s_cons (s_par p (p_ite e P Q)) M)
-                  (s_cons (s_par p P) M)
-  | f_cond: forall p e P Q M, 
-            eval_expr e = e_val (tbool false) ->
-            betaI (s_cons (s_par p (p_ite e P Q)) M)
-                  (s_cons (s_par p Q) M)
-  | r_struct: forall M1 M2 M1' M2',
-                     s_cong M1' M1 ->
-                     betaI M1 M2 ->
-                     s_cong M2 M2' ->
-                     betaI M1' M2'.
+Inductive multi {X : Type} (R : relation X) : relation X :=
+  | multi_refl : forall (x : X), multi R x x
+  | multi_step : forall (x y z : X), R x y -> multi R y z -> multi R x z.
+
+Definition beta_multistep := multi betaP.
+
+#[global] Declare Instance RW_scong3: Proper (scong ==> scong ==> impl) betaP.
+#[global] Declare Instance RW_scong4: Proper (scong ==> scong ==> impl) beta_multistep.
+
+Definition PAlice: process := 
+  p_send "Bob" "l1" (e_val (vint 50)) (p_recv "Carol" [("l3",sint,p_inact)]).
+
+Definition PBob: process :=
+  p_recv "Alice" [("l1",sint,p_send "Carol" "l2" (e_val (vint 100)) p_inact);
+                  ("l4",sint,p_send "Carol" "l2" (e_val (vint 2)) p_inact)
+                 ].
+
+Definition PCarol: process :=
+  p_recv "Bob" [("l2", sint, p_send "Alice" "l3" (e_plus (e_var 0) (e_val (vint 1))) p_inact)].
+
+Definition MS: session := ("Alice" <-- PAlice) ||| ("Bob" <-- PBob) ||| ("Carol" <-- PCarol).
+
+Definition MS': session := ("Alice" <-- p_inact) ||| ("Bob" <-- p_inact) ||| ("Carol" <-- p_inact).
+
+(* Eval compute in (eval_expr (e_plus (e_val (vint 100)) (e_val (vint 5)))). *)
+
+Example redMS: beta_multistep MS MS'.
+Proof. unfold beta_multistep, MS, MS', PAlice, PBob.
+
+       setoid_rewrite sc_par3.
+       setoid_rewrite sc_par2.
+       setoid_rewrite sc_par4.
+       setoid_rewrite <- sc_par3.
+
+       apply multi_step with
+       (y := ((("Bob" <-- p_send "Carol" "l2" (e_val (vint 100)) p_inact) |||
+              ("Alice" <-- (p_recv "Carol" [("l3", sint, p_inact)]))) ||| ("Carol" <-- PCarol))
+       ).
+       apply r_comm.
+       unfold PCarol.
+
+       setoid_rewrite sc_par2.
+       setoid_rewrite <- sc_par3.
+       apply multi_step with
+       (y := ((("Carol" <-- p_send "Alice" "l3" (e_plus (e_val (vint 100)) (e_val (vint 1)))  p_inact) |||
+              ("Bob" <-- p_inact)) ||| ("Alice" <-- p_recv "Carol" [("l3", sint, p_inact)]))
+       ).
+       apply r_comm.
+
+       setoid_rewrite sc_par2.
+       setoid_rewrite <- sc_par3.
+       apply multi_step with
+       (y := ((("Alice" <-- p_inact) |||
+              ("Carol" <-- p_inact)) ||| ("Bob" <-- p_inact))
+       ).
+       apply r_comm.
+       apply multi_refl.
+Qed.
+
+(*
+Definition PAliceT: process := 
+  p_rec (p_send "Bob" "l1" (e_val (vint 50%Z)) (p_recv "Carol" [("l3",sint,(p_var 0))])).
+
+Definition MSA (M: session): session := ("Alice" <-- PAliceT ||| M).
+
+Definition MSA' (M: session): session := ("Alice" <-- p_inact ||| M).
+
+Example redMSA: forall M, beta_multistep (MSA M) (MSA' M).
+Proof. unfold beta_multistep, MSA, MSA', PAliceT.
+       intro M.
+       rewrite sc_rec.
+ *)
+
+
+
