src/sessions.v
@@ -1,18 +1,26 @@
 From MPSTCoq Require Export src.unscoped src.expressions src.processes.
 Require Import List String Relations.
+Require Import List String Relations ZArith.
+Require Import Setoid Morphisms Coq.Program.Basics.
 
 Inductive session: Type :=
-  | s_par : part    -> process -> session
-  | s_cons: session -> session -> session.
+  | s_ind : part    -> process -> session
+  | s_par: session -> session -> session.
 
-Inductive s_cong: relation session :=
-  | s_cong_multi: forall P Q p M, 
-                  p_cong P Q -> 
-                  s_cong (s_cons (s_par p P) M) (s_cons (s_par p Q) M)
-  | s_cong_par1 : forall p M,
-                  s_cong (s_cons (s_par p p_inact) M) M
-  | s_cong_par2 : forall M M',
-                  s_cong (s_cons M M') (s_cons M' M)
-  | s_cong_par3 : forall M M' M'',
-                  s_cong (s_cons (s_cons M M') M'') (s_cons M (s_cons M' M'')).
+(* Inductive pcong: relation process :=
+  | pc_rec  : forall p, pcong (p_rec p) (subst_process ((p_rec p) .: p_var) p). *)
+
+Notation "p '<--' P"   :=  (s_ind p P) (at level 50, no associativity).
+Notation "s1 '|||' s2" :=  (s_par s1 s2) (at level 50, no associativity).
+
+Inductive scong: relation session :=
+  | sc_rec  : forall p P M, scong (p <-- (p_rec P) ||| M) (p <-- (subst_process ((p_rec P) .: p_var) P) ||| M)
+(*   | sc_multi: forall p P Q M, pcong P Q -> scong (p <-- P ||| M) (p <-- Q ||| M)  *)
+  | sc_par1 : forall p M, scong (p <-- p_inact ||| M) M
+  | sc_par2 : forall M M', scong (M ||| M') (M' ||| M)
+  | sc_par3 : forall M M' M'', scong ((M ||| M') ||| M'') (M ||| (M' ||| M''))
+  | sc_par4 : forall M M' M'', scong ((M ||| M') ||| M'') (M ||| (M'' ||| M')).
+
+(* Declare Instance Equivalence_pcong : Equivalence pcong. *)
+Declare Instance Equivalence_scong : Equivalence scong.
 
